\documentclass[12pt,a4paper]{article}
\usepackage[utf8]{inputenc}
\usepackage{amsmath}
\usepackage{amsfonts}
\usepackage{amssymb}
\usepackage{amsthm}
\usepackage{graphicx}
\author{Yusuf Brima}
\title{Linear Algebra}
\begin{document}
\section*{Exercise 3}
If  we have a linear model  
\begin{equation}
			\mathbf{y} =  \mathbf{w}  \cdot  \mathbf{x} 
\end{equation}
to show that 
\begin{equation}
    \mathbf{w}  =    \langle \mathbf{x}  \mathbf{x}   \rangle^{-1} \cdot    \langle \mathbf{x}  \mathbf{y} \rangle
\end{equation}
we define the mean squared loss as follow
\begin{equation}
	\mathcal{L}\left( \mathbf{x}^\mu  \mathbf{y}^\mu   \right) =  \frac{1}{2}  \sum_{\mu = 1}^n  \left(    \mathbf{y}^\mu   -  \mathbf{w} \cdot  \mathbf{x}^\mu   \right)^2
\end{equation}
where 
\begin{equation}
\langle \mathbf{x}  \mathbf{x}   \rangle :=  \frac{1}{n} \sum_{\mu = 1}^n  \mathbf{x}^\mu  \mathbf{x}^\mu
\end{equation}
and 
\begin{equation}
\langle \mathbf{x}  \mathbf{y}   \rangle :=  \frac{1}{n} \sum_{\mu = 1}^n  \mathbf{xy}^\mu  \mathbf{y}^\mu
\end{equation}
Solution
\begin{proof}
\begin{align*}
	\mathcal{L}\left( \mathbf{x}^\mu  \mathbf{y}^\mu   \right) &=  \frac{1}{2}  \sum_{\mu = 1}^n    \left(    \mathbf{y}^\mu   -  \mathbf{w} \cdot  \mathbf{x}^\mu   \right)^2\\
 \frac{\partial  \mathcal{L}  }{  \partial  \mathbf{w}  } &=   \frac{\partial  }{  \partial  \mathbf{w}  } \left(  \left(    \mathbf{y}^\mu   -  \mathbf{w} \cdot  \mathbf{x}^\mu   \right)^2     \right)\\
 &=  \frac{1}{2}  \left[    \left(    \mathbf{y}   -  \mathbf{w} \cdot  \mathbf{x}  \right)^2   +    \left(    \mathbf{y}^2   -  \mathbf{w} \cdot  \mathbf{x}^2  \right)^2 +  \cdots +  \left(    \mathbf{y}^n  -  \mathbf{w} \cdot  \mathbf{x}^n   \right)^2   \right]\\
 &=   -\mathbf{xy}  + \mathbf{wx^2}   -  \mathbf{x^2y^2} +  \cdots  +   \mathbf{x^ny^n}  + \mathbf{wx^{2n}} = 0\\
\mathbf{w}\left(   \mathbf{x^2}  + \mathbf{x^4}   +  \cdots  +  \mathbf{x^{2n}}  \right) &=  \mathbf{xy}  + \mathbf{x^2y^2} +  \cdots + \mathbf{x^ny^n}\\
\mathbf{w} &=  \frac{    \mathbf{xy}  + \mathbf{x^2y^2} +  \cdots + \mathbf{x^ny^n} }{ \left(   \mathbf{x^2}  + \mathbf{x^4}   +  \cdots  +  \mathbf{x^{2n}}  \right)}\\
\mathbf{w} &=  \frac{   \langle  \mathbf{xy} \rangle}{  \langle   \mathbf{xx} \rangle}\\
\therefore  \mathbf{w} &=   \langle   \mathbf{xx} \rangle^{-1}    \langle  \mathbf{xy} \rangle 
\end{align*}
\end{proof}
\end{document}